---
layout : post
pid : 25
title: "阿贝尔变换和分部积分"
date: 2020-06-19 15:59:13 +0800
cover_url: https://s2.banana.moe/unsplash_colle/romain-vignes-53940.jpg
category: Math
---

**部分和公式**

$$
\begin{align}
\sum_{i=m}^n a_{i+1}(b_{i+1}-b_i)+\sum_{i=m}^n b_{i}(a_{i+1}-a_i)=a_{n+1} b_{n+1}-a_m b_m
\end{align}
$$

这个公式在几何上是直观的:

![2020_06_23 上午11_55 Office Lens.jpg](http://ww1.sinaimg.cn/large/006bYYnlly1gg238agnwdj33sh1vtb29.jpg)

设 $f(x)\in R([x_0,x_n]),\quad g(x)\in R([y_0,y_n]),\quad f(x_i)=y_i,\quad g(y_i)=x_i,\quad\Delta f(x_i)=f(x_i)-f(x_{i-1})$

令$T_f=x_0<x_1<\cdots<x_{n-1}<x_n$ 为 $f$ 在 $[x_0,x_n]$ 上的一个分割,

令$T_g=y_0<y_1<\cdots<y_{n-1}<y_n$ 为 $g$ 在 $[y_0,y_n]$ 上的一个分割,

那么

$$
\sum_{i=0}^n f(x_{i+1})\Delta g(y_i)+\sum_{i=0}^n g(y_i)\Delta g(x_{i+1})=f(x_n)g(x_n)-f(x_0)g(x_0)
$$

令 $\lvert\lvert T_f\rvert\rvert\rightarrow0,\quad\lvert\lvert T_g\rvert\rvert\rightarrow0$ ,则

$$
\int_{y_0}^{y_n}f(x)dg(x)+\int_{x_0}^{x_n}g(x)df(x)=f(x_n)g(x_n)-f(x_0)g(x_0)
$$

此即分部求和公式:

$$
\int udv=uv-\int vdu
$$

令

$$
t_{i+1}=
\begin{cases}
b_{i+1}-b_i&i\geq m\\
0 & i<m
\end{cases}
$$

则$T_i=c_i$,整理可得

$$
\sum_{i=m}^n a_{i+1}t_{i+1}=\sum_{i=m}^n T_i(a_i-a_{i+1})+a_{n+1}T_{n+1}-a_m T_m
$$

此即Abel变换.




